

Homework 1

1. Let $F : \text{Mat}_{n \times n}(\mathbb{R}) \rightarrow \mathbb{R}$ be given by $F(A) := \det A$.

(a.) F is a polynomial in the n^2 entries of the matrix. It is thus differentiable as a map $\mathbb{R}^{n^2} \rightarrow \mathbb{R}$. The space \mathbb{R}^{n^2} is isomorphic to the space of $n \times n$ matrices as a finite dimensional normed vector space.

(b.) Suppose A is invertible. We are looking for a linear map $D_A F : \text{Mat}_{n \times n}(\mathbb{R}) \rightarrow \text{Mat}_{n \times n}(\mathbb{R})$ such that

$$F(A + H) = F(A) + D_A F(H) + r(H)$$

where $r(H) = o(\|H\|)$. We have

$$F(A + H) = \det(A + H) = \det(A) \det(I + A^{-1}H),$$

and we can write

$$\det(I + A^{-1}H) = 1 + \text{Tr}(A^{-1}H) + r(H),$$

where $r(H)$ consists of terms in the determinate of at least order 2 in the components of $A^{-1}H$.

We can bound $|r(H)|$ by a sum of absolute values of monics in elements of $A^{-1}H$ of orders at least 2. Then use $(A^{-1}H)_{ij} \leq \|A^{-1}H\| \leq \|A^{-1}\| \|H\|$, so that

$$\lim_{\|H\| \rightarrow 0} \frac{|r(H)|}{\|H\|} = 0.$$

Then we have

$$\det(A + H) = \det(A) + \det(A) \text{Tr}(A^{-1}H) + \det(A)r(H),$$

where of course the last term is still $o(\|H\|)$, and where $D_A F(H) = \det(A) \text{Tr}(A^{-1}H)$ is a linear map.

(c.) Using the formula for the inverse of an invertible matrix A , we have

$$D_A F(H) = \det(A) \text{Tr}(A^{-1}H) = \det(A) \frac{1}{\det(A)} \text{Tr}(\text{adj}(A)H) = \text{Tr}(\text{adj}(A)H).$$

Since the set of invertible matrices is dense in $\text{Mat}_{n \times n}(\mathbb{R})$, we can approach a non-invertible matrix B by a sequence of invertible matrices $\{A_j\}_{j=1}^\infty$ so that $A_j \rightarrow B$. Since F is continuously differentiable, $\lim_{j \rightarrow \infty} D_{A_j} F(H) = D_B F(H)$. Then $\lim_{j \rightarrow \infty} D_{A_j} F(H) = \lim_{j \rightarrow \infty} \text{Tr}(\text{adj}(A_j)H) = \text{Tr}(\text{adj} B)$, as trace and adjoint are both continuous functions.

2. Suppose $\Gamma : \mathbb{R} \rightarrow GL_n(\mathbb{R})$ is a smooth map such that $\Gamma(t)$ is orthogonal for every $t \in \mathbb{R}$. By the product rule, we have

$$\frac{d}{dt}(\Gamma(t)^T \Gamma(t)) = \frac{d}{dt}(\Gamma(t)^T) \Gamma(t) + \Gamma(t)^T \frac{d}{dt} \Gamma(t) = 0.$$

And we also see that

$$\frac{d}{dt}(\Gamma(t)^T) = \lim_{h \rightarrow 0} \frac{\Gamma(t+h)^T - \Gamma(t)^T}{h} = \lim_{h \rightarrow 0} \frac{(\Gamma(t+h) - \Gamma(t))^T}{h} = \left(\frac{d}{dt} \Gamma(t) \right)^T.$$

Then

$$\left(\Gamma(t)^{-1} \frac{d}{dt} \Gamma(t) \right)^T = \left(\Gamma(t)^T \frac{d}{dt} \Gamma(t) \right)^T = \left(\frac{d}{dt} \Gamma(t) \right)^T \Gamma(t) = -\Gamma(t)^T \frac{d}{dt} \Gamma(t) = -\Gamma(t)^{-1} \frac{d}{dt} \Gamma(t)$$

3. (a.) First we write down the action of $\widehat{V}_1 \circ \widehat{V}_2 - \widehat{V}_2 \circ \widehat{V}_1$ on a function $f \in C^\infty(U)$:

$$\begin{aligned}
\widehat{V}_1 \circ \widehat{V}_2 - \widehat{V}_2 \circ \widehat{V}_1(f) &= \widehat{V}_1 \left(\sum_{i=1}^n V_2^i \frac{\partial f}{\partial x_i} \right) - \widehat{V}_2 \left(\sum_{i=1}^n V_1^i \frac{\partial f}{\partial x_i} \right) \\
&= \sum_{j=1}^n \sum_{i=1}^n \left[V_1^j \frac{\partial V_2^i}{\partial x_j} \frac{\partial f}{\partial x_i} + V_1^j V_2^i \frac{\partial^2 f}{\partial x_j \partial x_i} \right] - \sum_{j=1}^n \sum_{i=1}^n V_2^j \left[\frac{\partial V_1^i}{\partial x_j} \frac{\partial f}{\partial x_i} + V_2^j V_1^i \frac{\partial^2 f}{\partial x_j \partial x_i} \right] \\
&= \sum_{j=1}^n \sum_{i=1}^n V_1^j \frac{\partial V_2^i}{\partial x_j} \frac{\partial f}{\partial x_i} - \sum_{j=1}^n \sum_{i=1}^n V_2^j \frac{\partial V_1^i}{\partial x_j} \frac{\partial f}{\partial x_i}. \\
&= \sum_{i=1}^n \sum_{j=1}^n V_1^j \frac{\partial V_2^i}{\partial x_j} \frac{\partial f}{\partial x_i} - \sum_{i=1}^n \sum_{j=1}^n V_2^j \frac{\partial V_1^i}{\partial x_j} \frac{\partial f}{\partial x_i}.
\end{aligned}$$

Then we see that $\widehat{V}_1 \circ \widehat{V}_2 - \widehat{V}_2 \circ \widehat{V}_1$ corresponds to a vector field W with components

$$W_i = \sum_{j=1}^n \left[V_1^j \frac{\partial V_2^i}{\partial x_j} - V_2^j \frac{\partial V_1^i}{\partial x_j} \right].$$

(b.) We calculate the Lie bracket of the vector fields $V_1 = \frac{\partial}{\partial x^1}$ and $V_2 = \frac{\partial}{\partial x^2} + (x^1)^2 \frac{\partial}{\partial x^3}$ to find

$$[V_1, V_2] = (2x^1) \frac{\partial}{\partial x^3}.$$

In order for $[V_1, V_2](x) \in \text{span}\{V_1(x), V_2(x)\}$, we need $a, b \in \mathbb{R}$ such that

$$(0, 0, 2x^1) = (a, b, b(x^1)^2),$$

which is only possible if $x = (0, 0, 0)$ and $a = b = 0$.

4. Assume the Implicit Function Theorem holds. Let $F : X \rightarrow Y$ be a C^1 map, where $X, Y \in \mathbb{R}^n$, and let $x_0 \in X, y_0 \in Y$ such that $y_0 = F(x_0)$, with $D_{x_0} F$ non-singular.

Define a new function $\tilde{F} : \mathbb{R}^n \times \mathbb{R}^n \rightarrow \mathbb{R}^n$ by $\tilde{F}(x, y) := F(x) - y$. Then $D_{x_0} \tilde{F}_1 = D_{x_0} F$, thus $D_{x_0} \tilde{F}_1$ is non-singular. By the Implicit Function Theorem in the first variable instead of the second, with $\tilde{F}(x_0, y_0) = 0 = z_0$, there exist neighborhoods $U \ni x_0$ and $V \ni y_0$ and a C^1 function $G : V \rightarrow U$ such that an element $(x, y) \in U \times V$ satisfies $\tilde{F}(x, y) = 0$ if and only if $x = G(y)$, and thus $F(x) = y$ if and only if $x = G(y)$. Then

$$F(G(y)) = y \quad G(F(x)) = x$$

for all $x \in U, y \in V$. Then it is clear that $G = F^{-1}$, and F is a C^1 diffeomorphism $U \rightarrow V$.